books/kestrel/remora/evaluation.lisp
@@ -46,7 +46,7 @@
                           var+typevalue-listp-when-result-not-error
                           typep-when-result-not-error
                           type-listp-when-result-not-error
-                          denvp-when-result-not-error)))
+                          expr-denvp-when-result-not-error)))
 
 ;;;;;;;;;;;;;;;;;;;;;;;;;;;;;;;;;;;;;;;;;;;;;;;;;;;;;;;;;;;;;;;;;;;;;;;;;;;;;;;;
 
@@ -68,7 +68,7 @@
 
   ;;;;;;;;;;;;;;;;;;;;;;;;;;;;;;;;;;;;;;;;
 
-  (define eval-dim ((dim dimp) (denv denvp))
+  (define eval-dim ((dim dimp) (denv expr-denvp))
     :returns (int integer-resultp)
     :parents (evaluation eval-dims)
     :short "Evaluate a dimension to an integer."
@@ -102,7 +102,7 @@
     (dim-case
      dim
      :var (b* (((ok val)
-                (denv-lookup-ispace-var (ispace-var-dim dim.name) denv))
+                (expr-denv-lookup-ispace (ispace-var-dim dim.name) denv))
                ((unless (ispace-value-case val :dim)) (reserr nil)))
             (ispace-value-dim->val val))
      :const dim.val
@@ -118,7 +118,7 @@
 
   ;;;;;;;;;;;;;;;;;;;;;;;;;;;;;;;;;;;;;;;;
 
-  (define eval-dim-list ((dims dim-listp) (denv denvp))
+  (define eval-dim-list ((dims dim-listp) (denv expr-denvp))
     :returns (ints integer-list-resultp)
     :parents (evaluation eval-dims)
     :short "Evaluate a list of dimensions to a list of integers."
@@ -163,7 +163,7 @@
 
   ;;;;;;;;;;;;;;;;;;;;;;;;;;;;;;;;;;;;;;;;
 
-  (define eval-shape ((shape shapep) (denv denvp))
+  (define eval-shape ((shape shapep) (denv expr-denvp))
     :returns (nats nat-list-resultp)
     :parents (evaluation eval-shapes/ispaces)
     :short "Evaluate a shape to a list of naturals."
@@ -201,7 +201,7 @@
     (shape-case
      shape
      :var (b* (((ok val)
-                (denv-lookup-ispace-var (ispace-var-shape shape.name) denv))
+                (expr-denv-lookup-ispace (ispace-var-shape shape.name) denv))
                ((unless (ispace-value-case val :shape)) (reserr nil)))
             (ispace-value-shape->val val))
      :dims (b* (((ok ints) (eval-dim-list shape.dims denv))
@@ -215,7 +215,7 @@
 
   ;;;;;;;;;;;;;;;;;;;;;;;;;;;;;;;;;;;;;;;;
 
-  (define eval-shape-list ((shapes shape-listp) (denv denvp))
+  (define eval-shape-list ((shapes shape-listp) (denv expr-denvp))
     :returns (natss nat-list-list-resultp)
     :parents (evaluation eval-shapes/ispaces)
     :short "Evaluate a list of shapes to a list of lists of naturals."
@@ -232,7 +232,7 @@
 
   ;;;;;;;;;;;;;;;;;;;;;;;;;;;;;;;;;;;;;;;;
 
-  (define eval-ispace ((ispace ispacep) (denv denvp))
+  (define eval-ispace ((ispace ispacep) (denv expr-denvp))
     :returns (ival ispace-value-resultp)
     :parents (evaluation eval-shapes/ispaces)
     :short "Evaluate an ispace to an ispace value."
@@ -254,7 +254,7 @@
 
   ;;;;;;;;;;;;;;;;;;;;;;;;;;;;;;;;;;;;;;;;
 
-  (define eval-ispace-list ((ispaces ispace-listp) (denv denvp))
+  (define eval-ispace-list ((ispaces ispace-listp) (denv expr-denvp))
     :returns (ivals ispace-value-list-resultp)
     :parents (evaluation eval-shapes/ispaces)
     :short "Evaluate a list of ispaces to a list of ispace values."
@@ -282,7 +282,7 @@
 
   ;;;;;;;;;;;;;;;;;;;;;;;;;;;;;;;;;;;;;;;;
 
-  (define eval-type ((type typep) (denv denvp))
+  (define eval-type ((type typep) (denv expr-denvp))
     :returns (tval type-value-resultp)
     :parents (evaluation eval-types)
     :short "Evaluate a type to a type value."
@@ -308,7 +308,7 @@
        They are treated like lambda abstractions."))
     (type-case
      type
-     :var (denv-lookup-type-var type.var denv)
+     :var (expr-denv-lookup-type type.var denv)
      :base (type-value-base type.type)
      :array (b* (((ok elem-tval) (eval-type type.elem denv))
                  ((ok ival) (eval-ispace type.ispace denv))
@@ -329,7 +329,7 @@
 
   ;;;;;;;;;;;;;;;;;;;;;;;;;;;;;;;;;;;;;;;;
 
-  (define eval-type-list ((types type-listp) (denv denvp))
+  (define eval-type-list ((types type-listp) (denv expr-denvp))
     :returns (tvals type-value-list-resultp)
     :parents (evaluation eval-types)
     :short "Evaluate a list of types to a list of type values."
@@ -367,7 +367,7 @@
 
 ;;;;;;;;;;;;;;;;;;;;;;;;;;;;;;;;;;;;;;;;;;;;;;;;;;;;;;;;;;;;;;;;;;;;;;;;;;;;;;;;
 
-(define eval-var+type? ((var+type? var+type?-p) (denv denvp))
+(define eval-var+type? ((var+type? var+type?-p) (denv expr-denvp))
   :returns (var+tval var+typevalue-resultp)
   :short "Evaluate a variable with an optional type
           to a variable with a type value."
@@ -382,7 +382,7 @@
 
 ;;;;;;;;;;;;;;;;;;;;;;;;;;;;;;;;;;;;;;;;
 
-(define eval-var+type?-list ((var+types var+type?-listp) (denv denvp))
+(define eval-var+type?-list ((var+types var+type?-listp) (denv expr-denvp))
   :returns (var+tvals var+typevalue-list-resultp)
   :short "Evaluate a list of variables with optional types
           to a list of variables with type values."
@@ -1032,8 +1032,8 @@
 
   ;;;;;;;;;;;;;;;;;;;;;;;;;;;;;;;;;;;;;;;;
 
-  (define eval-expr ((expr exprp) (denv denvp) (limit natp))
-    :guard (denv-wfp denv)
+  (define eval-expr ((expr exprp) (denv expr-denvp) (limit natp))
+    :guard (expr-denv-wfp denv)
     :returns (val expr-value-resultp)
     :parents (evaluation eval-exprs/atoms/binds)
     :short "Evaluate an expression to an expression value."
@@ -1136,7 +1136,7 @@
     (b* (((when (zp limit)) (reserr :limit)))
       (expr-case
        expr
-       :var (denv-lookup-expr-var expr.name denv)
+       :var (expr-denv-lookup-expr expr.name denv)
        :atom (eval-atom expr.atom denv (1- limit))
        :array (b* (((when (member-equal 0 expr.dims)) (reserr nil))
                    ((ok vals) (eval-atom-list expr.atoms denv (1- limit)))
@@ -1222,8 +1222,8 @@
 
   ;;;;;;;;;;;;;;;;;;;;;;;;;;;;;;;;;;;;;;;;
 
-  (define eval-expr-list ((exprs expr-listp) (denv denvp) (limit natp))
-    :guard (denv-wfp denv)
+  (define eval-expr-list ((exprs expr-listp) (denv expr-denvp) (limit natp))
+    :guard (expr-denv-wfp denv)
     :returns (vals expr-value-list-resultp)
     :parents (evaluation eval-exprs/atoms/binds)
     :short "Evaluate a list of expressions to a list of expression values."
@@ -1251,8 +1251,8 @@
 
   ;;;;;;;;;;;;;;;;;;;;;;;;;;;;;;;;;;;;;;;;
 
-  (define eval-atom ((atom atomp) (denv denvp) (limit natp))
-    :guard (denv-wfp denv)
+  (define eval-atom ((atom atomp) (denv expr-denvp) (limit natp))
+    :guard (expr-denv-wfp denv)
     :returns (val expr-value-resultp)
     :parents (evaluation eval-exprs/atoms/binds)
     :short "Evaluate an atom to an expression value."
@@ -1304,8 +1304,8 @@
 
   ;;;;;;;;;;;;;;;;;;;;;;;;;;;;;;;;;;;;;;;;
 
-  (define eval-atom-list ((atoms atom-listp) (denv denvp) (limit natp))
-    :guard (denv-wfp denv)
+  (define eval-atom-list ((atoms atom-listp) (denv expr-denvp) (limit natp))
+    :guard (expr-denv-wfp denv)
     :returns (vals expr-value-list-resultp)
     :parents (evaluation eval-exprs/atoms/binds)
     :short "Evaluate a list of atoms to a list of expression values."
@@ -1333,9 +1333,9 @@
 
   ;;;;;;;;;;;;;;;;;;;;;;;;;;;;;;;;;;;;;;;;
 
-  (define eval-bind ((bind bindp) (denv denvp) (limit natp))
-    :guard (denv-wfp denv)
-    :returns (new-denv denv-resultp)
+  (define eval-bind ((bind bindp) (denv expr-denvp) (limit natp))
+    :guard (expr-denv-wfp denv)
+    :returns (new-denv expr-denv-resultp)
     :parents (evaluation eval-exprs/atoms/binds)
     :short "Evaluate a binding, extending the dynamic environment."
     :long
@@ -1415,15 +1415,15 @@
       (bind-case
        bind
        :ispace (b* (((ok ival) (eval-ispace bind.ispace denv)))
-                 (denv-add-ispace-var bind.var ival denv))
+                 (expr-denv-add-ispace bind.var ival denv))
        :type (b* (((ok tval) (eval-type bind.type denv)))
-               (denv-add-type-var bind.var tval denv))
+               (expr-denv-add-type bind.var tval denv))
        :val (b* (((ok val) (eval-expr bind.expr denv (1- limit)))
                  ((ok &) (type-option-case
                           bind.type?
                           :some (eval-type bind.type?.val denv)
                           :none nil)))
-              (denv-add-expr-var bind.var val denv))
+              (expr-denv-add-expr bind.var val denv))
        :fun (b* (((ok params) (eval-var+type?-list bind.params denv))
                  (val (make-expr-value-lambda :params params
                                               :body bind.expr
@@ -1432,7 +1432,7 @@
                           bind.type?
                           :some (eval-type bind.type?.val denv)
                           :none nil)))
-              (denv-add-expr-var bind.var val denv))
+              (expr-denv-add-expr bind.var val denv))
        :tfun (b* ((val (make-expr-value-tlambda :params bind.params
                                                 :body bind.expr))
                   ((ok &) (type-option-case
@@ -1442,7 +1442,7 @@
                                                     :body bind.type?.val)
                                   denv)
                            :none nil)))
-               (denv-add-expr-var bind.var val denv))
+               (expr-denv-add-expr bind.var val denv))
        :ifun (b* ((val (make-expr-value-ilambda :params bind.params
                                                 :body bind.expr))
                   ((ok &) (type-option-case
@@ -1452,7 +1452,7 @@
                                                 :body bind.type?.val)
                                   denv)
                            :none nil)))
-               (denv-add-expr-var bind.var val denv))
+               (expr-denv-add-expr bind.var val denv))
        :cfun (b* ((lambda-expr (make-expr-array
                                 :dims nil
                                 :atoms (list (make-atom-lambda
@@ -1487,14 +1487,14 @@
                     :none (mv iexpr itype)))
                   ((ok val) (eval-expr cfun-expr denv (1- limit)))
                   ((ok &) (eval-type cfun-type denv)))
-               (denv-add-expr-var bind.var val denv))))
+               (expr-denv-add-expr bind.var val denv))))
     :measure (nfix limit))
 
   ;;;;;;;;;;;;;;;;;;;;;;;;;;;;;;;;;;;;;;;;
 
-  (define eval-bind-list ((binds bind-listp) (denv denvp) (limit natp))
-    :guard (denv-wfp denv)
-    :returns (new-denv denv-resultp)
+  (define eval-bind-list ((binds bind-listp) (denv expr-denvp) (limit natp))
+    :guard (expr-denv-wfp denv)
+    :returns (new-denv expr-denv-resultp)
     :parents (evaluation eval-exprs/atoms/binds)
     :short "Evaluate a list of bindings,
             threading the dynamic environment through them."
@@ -1505,7 +1505,7 @@
        extending the dynamic environment as we go,
        and we return the final environment."))
     (b* (((when (zp limit)) (reserr :limit))
-         ((when (endp binds)) (denv-fix denv))
+         ((when (endp binds)) (expr-denv-fix denv))
          ((ok denv) (eval-bind (car binds) denv (1- limit))))
       (eval-bind-list (cdr binds) denv (1- limit)))
     :measure (nfix limit))
@@ -1514,10 +1514,10 @@
 
   (define eval-tapp ((funval expr-valuep)
                      (tvals type-value-listp)
-                     (denv denvp)
+                     (denv expr-denvp)
                      (limit natp))
     :guard (and (expr-value-wfp funval)
-                (denv-wfp denv))
+                (expr-denv-wfp denv))
     :returns (val expr-value-resultp)
     :parents (evaluation eval-exprs/atoms/binds)
     :short "Apply an expression value to type values."
@@ -1585,7 +1585,7 @@
        :tlambda
        (b* (((unless (type-values-match-type-vars-p tvals funval.params))
              (reserr nil))
-            (denv (denv-add-type-vars funval.params tvals denv)))
+            (denv (expr-denv-add-types funval.params tvals denv)))
          (eval-expr funval.body denv (1- limit)))
        :primop (if (primop-value-tfunp funval.val)
                    (eval-primop-tfun funval.val tvals)
@@ -1602,7 +1602,7 @@
         :forall
         (b* (((unless (type-values-match-type-vars-p tvals funval.elem.params))
               (reserr nil))
-             (denv (denv-add-type-vars funval.elem.params tvals denv))
+             (denv (expr-denv-add-types funval.elem.params tvals denv))
              ((ok tval) (eval-type funval.elem.body denv))
              ((mv elem body-dims)
               (type-value-case
@@ -1620,10 +1620,10 @@
 
   (define eval-tapp-list ((funvals expr-value-listp)
                           (tvals type-value-listp)
-                          (denv denvp)
+                          (denv expr-denvp)
                           (limit natp))
     :guard (and (expr-value-list-wfp funvals)
-                (denv-wfp denv))
+                (expr-denv-wfp denv))
     :returns (vals expr-value-list-resultp)
     :parents (evaluation eval-exprs/atoms/binds)
     :short "Lift @(tsee eval-tapp) to a list of function values."
@@ -1655,10 +1655,10 @@
 
   (define eval-iapp ((funval expr-valuep)
                      (ivals ispace-value-listp)
-                     (denv denvp)
+                     (denv expr-denvp)
                      (limit natp))
     :guard (and (expr-value-wfp funval)
-                (denv-wfp denv))
+                (expr-denv-wfp denv))
     :returns (val expr-value-resultp)
     :parents (evaluation eval-exprs/atoms/binds)
     :short "Apply an expression value to ispace values."
@@ -1726,7 +1726,7 @@
        :ilambda
        (b* (((unless (ispace-values-match-ispace-vars-p ivals funval.params))
              (reserr nil))
-            (denv (denv-add-ispace-vars funval.params ivals denv)))
+            (denv (expr-denv-add-ispaces funval.params ivals denv)))
          (eval-expr funval.body denv (1- limit)))
        :primop (if (primop-value-ifunp funval.val)
                    (eval-primop-ifun funval.val ivals)
@@ -1744,7 +1744,7 @@
         (b* (((unless (ispace-values-match-ispace-vars-p ivals
                                                          funval.elem.params))
               (reserr nil))
-             (denv (denv-add-ispace-vars funval.elem.params ivals denv))
+             (denv (expr-denv-add-ispaces funval.elem.params ivals denv))
              ((ok tval) (eval-type funval.elem.body denv))
              ((mv elem body-dims)
               (type-value-case
@@ -1762,10 +1762,10 @@
 
   (define eval-iapp-list ((funvals expr-value-listp)
                           (ivals ispace-value-listp)
-                          (denv denvp)
+                          (denv expr-denvp)
                           (limit natp))
     :guard (and (expr-value-list-wfp funvals)
-                (denv-wfp denv))
+                (expr-denv-wfp denv))
     :returns (vals expr-value-list-resultp)
     :parents (evaluation eval-exprs/atoms/binds)
     :short "Lift @(tsee eval-iapp) to a list of function values."
@@ -1797,11 +1797,11 @@
 
   (define eval-app ((funval expr-valuep)
                     (argvals expr-value-listp)
-                    (denv denvp)
+                    (denv expr-denvp)
                     (limit natp))
     :guard (and (expr-value-wfp funval)
                 (expr-value-list-wfp argvals)
-                (denv-wfp denv))
+                (expr-denv-wfp denv))
     :returns (val expr-value-resultp)
     :parents (evaluation eval-exprs/atoms/binds)
     :short "Apply an expression value to argument expression values."
@@ -1913,9 +1913,9 @@
 
   (define eval-app-list ((funcells expr-value-listp)
                          (argcell-lists expr-value-list-listp)
-                         (denv denvp)
+                         (denv expr-denvp)
                          (limit natp))
-    :guard (denv-wfp denv)
+    :guard (expr-denv-wfp denv)
     :returns (vals expr-value-list-resultp)
     :parents (evaluation eval-exprs/atoms/binds)
     :short "Apply function cells to argument cells, position-wise."
@@ -1955,10 +1955,10 @@
 
   (define eval-app-cell ((funcell expr-valuep)
                          (argcells expr-value-listp)
-                         (denv denvp)
+                         (denv expr-denvp)
                          (limit natp))
     :guard (and (expr-value-list-wfp argcells)
-                (denv-wfp denv))
+                (expr-denv-wfp denv))
     :returns (val expr-value-resultp)
     :parents (evaluation eval-exprs/atoms/binds)
     :short "Apply a single (scalar) function cell to its argument cells."
@@ -1988,7 +1988,7 @@
                       argcells
                       (var+typevalue-list->type funcell.params)))
              (reserr nil))
-            (denv (denv-add-expr-vars
+            (denv (expr-denv-add-exprs
                    (var+typevalue-list->var funcell.params)
                    argcells
                    denv)))
@@ -2006,10 +2006,10 @@
                       (var stringp)
                       (body exprp)
                       (type type-valuep)
-                      (denv denvp)
+                      (denv expr-denvp)
                       (limit natp))
     :guard (and (expr-value-wfp target)
-                (denv-wfp denv))
+                (expr-denv-wfp denv))
     :returns (val expr-value-resultp)
     :parents (evaluation eval-exprs/atoms/binds)
     :short "Evaluate the unboxing of a target value."
@@ -2056,8 +2056,8 @@
        :box
        (b* (((unless (ispace-values-match-ispace-vars-p target.ispaces ispaces))
              (reserr nil))
-            (denv (denv-add-ispace-vars ispaces target.ispaces denv))
-            (denv (denv-add-expr-var var target.array denv)))
+            (denv (expr-denv-add-ispaces ispaces target.ispaces denv))
+            (denv (expr-denv-add-expr var target.array denv)))
          (eval-expr body denv (1- limit)))
        :vector
        (b* (((ok vals)
@@ -2085,10 +2085,10 @@
                            (var stringp)
                            (body exprp)
                            (type type-valuep)
-                           (denv denvp)
+                           (denv expr-denvp)
                            (limit natp))
     :guard (and (expr-value-list-wfp targets)
-                (denv-wfp denv))
+                (expr-denv-wfp denv))
     :returns (vals expr-value-list-resultp)
     :parents (evaluation eval-exprs/atoms/binds)
     :short "Lift @(tsee eval-unbox) to a list of target values."
@@ -2131,47 +2131,47 @@
     :hints (("Goal"
              :expand ((eval-expr expr denv limit)
                       (eval-expr (expr-fix expr) denv limit)
-                      (eval-expr expr (denv-fix denv) limit)
+                      (eval-expr expr (expr-denv-fix denv) limit)
                       (eval-expr-list exprs denv limit)
                       (eval-expr-list (expr-list-fix exprs) denv limit)
-                      (eval-expr-list exprs (denv-fix denv) limit)
+                      (eval-expr-list exprs (expr-denv-fix denv) limit)
                       (eval-atom atom denv limit)
                       (eval-atom (atom-fix atom) denv limit)
-                      (eval-atom atom (denv-fix denv) limit)
+                      (eval-atom atom (expr-denv-fix denv) limit)
                       (eval-atom-list atoms denv limit)
                       (eval-atom-list (atom-list-fix atoms) denv limit)
-                      (eval-atom-list atoms (denv-fix denv) limit)
+                      (eval-atom-list atoms (expr-denv-fix denv) limit)
                       (eval-bind bind denv limit)
                       (eval-bind (bind-fix bind) denv limit)
-                      (eval-bind bind (denv-fix denv) limit)
+                      (eval-bind bind (expr-denv-fix denv) limit)
                       (eval-bind-list binds denv limit)
                       (eval-bind-list (bind-list-fix binds) denv limit)
-                      (eval-bind-list binds (denv-fix denv) limit)
+                      (eval-bind-list binds (expr-denv-fix denv) limit)
                       (eval-tapp funval tvals denv limit)
                       (eval-tapp (expr-value-fix funval) tvals denv limit)
                       (eval-tapp funval (type-value-list-fix tvals) denv limit)
-                      (eval-tapp funval tvals (denv-fix denv) limit)
+                      (eval-tapp funval tvals (expr-denv-fix denv) limit)
                       (eval-tapp-list funvals tvals denv limit)
                       (eval-tapp-list (expr-value-list-fix funvals)
                                       tvals denv limit)
                       (eval-tapp-list funvals
                                       (type-value-list-fix tvals) denv limit)
-                      (eval-tapp-list funvals tvals (denv-fix denv) limit)
+                      (eval-tapp-list funvals tvals (expr-denv-fix denv) limit)
                       (eval-iapp funval ivals denv limit)
                       (eval-iapp (expr-value-fix funval) ivals denv limit)
                       (eval-iapp funval
                                  (ispace-value-list-fix ivals) denv limit)
-                      (eval-iapp funval ivals (denv-fix denv) limit)
+                      (eval-iapp funval ivals (expr-denv-fix denv) limit)
                       (eval-iapp-list funvals ivals denv limit)
                       (eval-iapp-list (expr-value-list-fix funvals)
                                       ivals denv limit)
                       (eval-iapp-list funvals
                                       (ispace-value-list-fix ivals) denv limit)
-                      (eval-iapp-list funvals ivals (denv-fix denv) limit)
+                      (eval-iapp-list funvals ivals (expr-denv-fix denv) limit)
                       (eval-app funval argvals denv limit)
                       (eval-app (expr-value-fix funval) argvals denv limit)
                       (eval-app funval (expr-value-list-fix argvals) denv limit)
-                      (eval-app funval argvals (denv-fix denv) limit)
+                      (eval-app funval argvals (expr-denv-fix denv) limit)
                       (eval-app-list funcells argcell-lists denv limit)
                       (eval-app-list (expr-value-list-fix funcells)
                                      argcell-lists denv limit)
@@ -2179,12 +2179,12 @@
                                      (expr-value-list-list-fix argcell-lists)
                                      denv limit)
                       (eval-app-list funcells argcell-lists
-                                     (denv-fix denv) limit)
+                                     (expr-denv-fix denv) limit)
                       (eval-app-cell funcell argcells denv limit)
                       (eval-app-cell (expr-value-fix funcell) argcells denv limit)
                       (eval-app-cell funcell (expr-value-list-fix argcells)
                                      denv limit)
-                      (eval-app-cell funcell argcells (denv-fix denv) limit)
+                      (eval-app-cell funcell argcells (expr-denv-fix denv) limit)
                       (eval-unbox target ispaces var body type denv limit)
                       (eval-unbox (expr-value-fix target)
                                   ispaces var body type denv limit)
@@ -2197,7 +2197,7 @@
                       (eval-unbox target ispaces var body
                                   (type-value-fix type) denv limit)
                       (eval-unbox target ispaces var body
-                                  type (denv-fix denv) limit)
+                                  type (expr-denv-fix denv) limit)
                       (eval-unbox-list targets ispaces var body type denv limit)
                       (eval-unbox-list (expr-value-list-fix targets)
                                        ispaces var body type denv limit)
@@ -2210,86 +2210,86 @@
                       (eval-unbox-list targets ispaces var body
                                        (type-value-fix type) denv limit)
                       (eval-unbox-list targets ispaces var body
-                                       type (denv-fix denv) limit))
+                                       type (expr-denv-fix denv) limit))
              :in-theory (enable nfix zp))))
 
   ;;;;;;;;;;;;;;;;;;;;;;;;;;;;;;;;;;;;;;;;
 
   (defret-mutual expr-value-wfp-of-eval-exprs/atoms/binds
     (defret expr-value-wfp-of-eval-expr
-      (implies (and (denv-wfp denv)
+      (implies (and (expr-denv-wfp denv)
                     (not (reserrp val)))
                (expr-value-wfp val))
       :fn eval-expr)
     (defret expr-value-list-wfp-of-eval-expr-list
-      (implies (and (denv-wfp denv)
+      (implies (and (expr-denv-wfp denv)
                     (not (reserrp vals)))
                (expr-value-list-wfp vals))
       :fn eval-expr-list)
     (defret expr-value-wfp-of-eval-atom
-      (implies (and (denv-wfp denv)
+      (implies (and (expr-denv-wfp denv)
                     (not (reserrp val)))
                (expr-value-wfp val))
       :fn eval-atom)
     (defret expr-value-list-wfp-of-eval-atom-list
-      (implies (and (denv-wfp denv)
+      (implies (and (expr-denv-wfp denv)
                     (not (reserrp vals)))
                (expr-value-list-wfp vals))
       :fn eval-atom-list)
-    (defret denv-wfp-of-eval-bind
-      (implies (and (denv-wfp denv)
+    (defret expr-denv-wfp-of-eval-bind
+      (implies (and (expr-denv-wfp denv)
                     (not (reserrp new-denv)))
-               (denv-wfp new-denv))
+               (expr-denv-wfp new-denv))
       :fn eval-bind)
-    (defret denv-wfp-of-eval-bind-list
-      (implies (and (denv-wfp denv)
+    (defret expr-denv-wfp-of-eval-bind-list
+      (implies (and (expr-denv-wfp denv)
                     (not (reserrp new-denv)))
-               (denv-wfp new-denv))
+               (expr-denv-wfp new-denv))
       :fn eval-bind-list)
     (defret expr-value-wfp-of-eval-tapp
-      (implies (and (denv-wfp denv)
+      (implies (and (expr-denv-wfp denv)
                     (not (reserrp val)))
                (expr-value-wfp val))
       :fn eval-tapp)
     (defret expr-value-list-wfp-of-eval-tapp-list
-      (implies (and (denv-wfp denv)
+      (implies (and (expr-denv-wfp denv)
                     (not (reserrp vals)))
                (expr-value-list-wfp vals))
       :fn eval-tapp-list)
     (defret expr-value-wfp-of-eval-iapp
-      (implies (and (denv-wfp denv)
+      (implies (and (expr-denv-wfp denv)
                     (not (reserrp val)))
                (expr-value-wfp val))
       :fn eval-iapp)
     (defret expr-value-list-wfp-of-eval-iapp-list
-      (implies (and (denv-wfp denv)
+      (implies (and (expr-denv-wfp denv)
                     (not (reserrp vals)))
                (expr-value-list-wfp vals))
       :fn eval-iapp-list)
     (defret expr-value-wfp-of-eval-app
-      (implies (and (denv-wfp denv)
+      (implies (and (expr-denv-wfp denv)
                     (not (reserrp val)))
                (expr-value-wfp val))
       :fn eval-app)
     (defret expr-value-list-wfp-of-eval-app-list
-      (implies (and (denv-wfp denv)
+      (implies (and (expr-denv-wfp denv)
                     (not (reserrp vals)))
                (expr-value-list-wfp vals))
       :fn eval-app-list)
     (defret expr-value-wfp-of-eval-app-cell
-      (implies (and (denv-wfp denv)
+      (implies (and (expr-denv-wfp denv)
                     (expr-value-list-wfp argcells)
                     (not (reserrp val)))
                (expr-value-wfp val))
       :fn eval-app-cell)
     (defret expr-value-wfp-of-eval-unbox
-      (implies (and (denv-wfp denv)
+      (implies (and (expr-denv-wfp denv)
                     (expr-value-wfp target)
                     (not (reserrp val)))
                (expr-value-wfp val))
       :fn eval-unbox)
     (defret expr-value-list-wfp-of-eval-unbox-list
-      (implies (and (denv-wfp denv)
+      (implies (and (expr-denv-wfp denv)
                     (expr-value-list-wfp targets)
                     (not (reserrp vals)))
                (expr-value-list-wfp vals))
@@ -2297,7 +2297,7 @@
     :mutual-recursion eval-exprs/atoms/binds
     :hints
     (("Goal"
-      :in-theory (enable expr-value-wfp-of-cdr-of-assoc-when-denv-wfp
+      :in-theory (enable expr-value-wfp-of-cdr-of-assoc-when-expr-denv-wfp
                          expr-value-wfp-of-expr-value-with-nonempty-dims
                          nfix
                          zp)
